examples/computability/turingMachines/turing_machine_primeqScript.sml
@@ -1,4 +1,5 @@
 
+
 open HolKernel Parse boolLib bossLib finite_mapTheory;
 open recfunsTheory;
 open recursivefnsTheory;
@@ -18,7 +19,7 @@ val updn_def = Define `(updn [] = 0) ∧ (updn [x] = tri x) ∧
                 else if y = 1 then tri (x + 2) + 2
                 else if y = 2 then tri x
                 else nB (y = 3) * tri x) ∧
- (updn [s;actn;tmn] =
+ (updn [s;actn;tmn] = 
   let tape = (nsnd tmn) in
   let tl = (nfst tape) in
   let th = ((nsnd tape) MOD 2) in
@@ -430,20 +431,16 @@ SRW_TAC [][updn_def,primrec_rules,prim_pr_rec_updn] >> SRW_TAC [][pr_cond_def] >
 
 
 val tmstepf_def = tDefine "tmstepf" `tmstepf p tmn =
-     case OLEAST n. (NUM_TO_STATE (nfst n), CELL_NUM (nsnd n)) ∈ FDOM p of
-         NONE => (tmn)
+     case OLEAST n. ((NUM_TO_STATE (nfst n), CELL_NUM (nsnd n)) ∈ FDOM p) ∧ (nfst n<>0) of
+         NONE => 0 *, nsnd tmn
        | SOME n => let s = NUM_TO_STATE (nfst n) in
-                       let sym = CELL_NUM (nsnd n) in
-                   let (s',actn) = p ' (s,sym) in
+                   let sym = CELL_NUM (nsnd n) in
+                   let (s',actn) = p ' (s,sym) in  if nfst n = 0 then tmn else
         ( if ((nfst tmn) = STATE_TO_NUM s) ∧ (((nsnd (nsnd tmn)) MOD 2) = NUM_CELL sym)
           then updn [STATE_TO_NUM s'; ACT_TO_NUM actn; tmn]
           else tmstepf (p \\ (s,sym)) tmn
           )` (WF_REL_TAC `measure (CARD o FDOM o FST)` >> simp[OLEAST_EQ_SOME] >>
                      metis_tac[MEMBER_CARD]);
-
-
-
-
 
 val HEAD_DECODE_ENCDOE_EQ = Q.store_thm("HEAD_DECODE_ENCDOE_EQ[simp]",
 `(HD (DECODE (ENCODE t)) = Z) ==> (HD t = Z)`,
@@ -527,7 +524,7 @@ val lemma_11 = UPDATE_TM_ARB_Q |> Q.INST[`q` |-> `tm.prog` ]  |> SIMP_RULE(srw_s
 
 
 val updn_UPDATE_TAPE = Q.store_thm("updn_UPDATE_TAPE",
-`((tm.state, tm.tape_h) ∈ FDOM p) ==> ((λ(s',actn). updn [STATE_TO_NUM s'; ACT_TO_NUM actn; ⟦tm⟧])
+`((tm.state, tm.tape_h) ∈ FDOM p) ∧ (tm.state.n <> 0) ==> ((λ(s',actn). updn [STATE_TO_NUM s'; ACT_TO_NUM actn; ⟦tm⟧])
  (p ' (tm.state,tm.tape_h)) = ⟦UPDATE_TAPE (tm with prog := p)⟧)`,
 rw[] >> `ACT_TO_NUM actn < 4` by fs[ACT_TO_NUM_LESS_4] >>
 `(tm.state,tm.tape_h) ∈ FDOM (tm with prog := p).prog` by fs[] >>
@@ -572,37 +569,152 @@ simp[DOMSUB_FAPPLY_THM] )
 
 
 val UPDATE_W_PROG_NIN_TM = Q.store_thm("UPDATE_W_PROG_NIN_TM",
-`((NUM_CELL (CELL_NUM c) = c) ∧ ((NUM_TO_STATE n,CELL_NUM c) ∈ FDOM p) ∧
+`((NUM_CELL (CELL_NUM c) = c) ∧ ((NUM_TO_STATE n,CELL_NUM c) ∈ FDOM p) ∧ (n <> 0) ∧
   ((STATE_TO_NUM tm.state = n) ⇒ NUM_CELL tm.tape_h ≠ c))
   ⇒ (⟦UPDATE_TAPE (tm with prog := p \\ (NUM_TO_STATE n,CELL_NUM c)) ⟧ =
   ⟦UPDATE_TAPE (tm with prog := p)⟧)`,
-rw[] >> simp[FULL_ENCODE_TM_def]  >>
+ simp[FULL_ENCODE_TM_def]  >> rw[] >>
 `(tm.state = NUM_TO_STATE n) ⇒ tm.tape_h ≠ CELL_NUM c` by metis_tac[NUM_STATE_CELL_NUM_LEM] >>
 `(tm.state,tm.tape_h) <> (NUM_TO_STATE n,CELL_NUM c)` by fs[] >>
-rw[] >> Cases_on `((tm.state,tm.tape_h) ∈ FDOM p)` >> fs[UPDATE_TAPE_def] >> fs[EQ_SND_P_LESS] >>
+rw[] >> Cases_on `((tm.state,tm.tape_h) ∈ FDOM p)` >> rw[UPDATE_TAPE_def] >> fs[EQ_SND_P_LESS] >>
 Cases_on `SND (p ' (tm.state,tm.tape_h))` >> fs[] >> Cases_on `tm.tape_l = []` >> fs[] >>
 Cases_on `tm.tape_r = []` >> fs[ENCODE_TM_TAPE_def] )
+
+val tm_eq_tm_with_state = Q.store_thm("tm_eq_tm_with_state",
+`(tm.state = a) ==> (tm = tm with state := a)`,
+strip_tac >> `(tm with state := a).state = a` by fs[] >> rfs[TM_component_equality])
+
+val effempty_def = Define`effempty p <=> FDOM p ⊆ {(a:state,b) | (a,b) | a = 0}`
+
+val containment_lem_nzero = Q.store_thm("tm_eq_tm_with_state",
+`(((OLEAST n. (NUM_TO_STATE (nfst n),CELL_NUM (nsnd n)) ∈ FDOM p ∧
+                              (nfst n <>0))  =  NONE) ⇔ effempty p)`,
+rw[oleast_eq_none,effempty_def] >> eq_tac >> simp[] >> csimp[fmap_EXT] >>
+simp[EXTENSION,pairTheory.FORALL_PROD,NUM_TO_STATE_def] >> strip_tac
+>- (rw[SUBSET_DEF] >> rename[`sc ∈ FDOM p`] >> `∃s c. sc = (s,c)` by simp[pairTheory.pair_CASES]>>
+    rw[] >> first_x_assum (qspec_then `s.n *, (NUM_CELL c)` mp_tac) >>simp[]>>
+    `<|n := s.n|> = s` by (simp[state_component_equality]) >> simp[state_component_equality,st_def])
+>- (rpt strip_tac >> fs[SUBSET_DEF] >> res_tac >> fs[st_def]) );
+
+
+
+val effempty_no_update = Q.store_thm("effempty_no_update",
+`effempty tm.prog ==> (UPDATE_TAPE tm = tm with state := <|n := 0|>)`,
+rw[effempty_def]>> simp[UPDATE_TAPE_def]>> Cases_on `(tm.state,tm.tape_h) ∈ FDOM tm.prog`>> simp[]>>
+  fs[SUBSET_DEF] >> res_tac >> fs[st_def])
+
+
+val CELL_NUM_LEM11 = Q.store_thm("CELL_NUM_LEM1",
+`((∀n'. n' < n ⊗ c ⇒ nfst n' ≠ 0 ⇒ (NUM_TO_STATE (nfst n'),CELL_NUM (nsnd n')) ∉ FDOM p )
+      ∧ ( (NUM_TO_STATE n,CELL_NUM c) ∈ FDOM p) ∧ n<>0) ==> ((c=0) ∨ (c=1))`,
+spose_not_then strip_assume_tac >> Cases_on `CELL_NUM c` >-
+               (`0<c` by simp[] >> metis_tac[nfst_npair,nsnd_npair,npair_mono,CELL_NUM_def]  ) >-
+               (`1<c` by simp[] >> metis_tac[nfst_npair,nsnd_npair,npair_mono,CELL_NUM_def]  ) );
+
+val FULL_ENCODE_IGNORES_PROGS' = FULL_ENCODE_IGNORES_PROGS |> SYM  |> Q.INST[`p`|->`ARB` ]
 
 val tmstepf_update_equiv = Q.store_thm("tmstepf_update_equiv",
 `∀p n tm. (n = ⟦tm⟧ ) ==>
         (tmstepf p n = FULL_ENCODE_TM (UPDATE_TAPE (tm with prog := p) ))`,
 ho_match_mp_tac (theorem"tmstepf_ind") >> simp[OLEAST_EQ_SOME] >> rw[] >>
 pop_assum (assume_tac o CONV_RULE (HO_REWR_CONV npair_lem)) >> fs[] >> simp[Once tmstepf_def] >>
-Cases_on `OLEAST n. (NUM_TO_STATE (nfst n),CELL_NUM (nsnd n)) ∈ FDOM p`
->- (simp[] >> fs[containment_lem]  >> simp[UPDATE_TAPE_def] )
+Cases_on `OLEAST n. (NUM_TO_STATE (nfst n),CELL_NUM (nsnd n)) ∈ FDOM p ∧ nfst n ≠ 0`
+>- (simp[] >> fs[containment_lem_nzero,effempty_no_update] >>
+    simp[UPDATE_TAPE_def,FULL_ENCODE_TM_def,STATE_TO_NUM_def,ENCODE_TM_TAPE_def] )
 >- (fs[OLEAST_EQ_SOME] >> rename [`NUM_TO_STATE (nfst nc)`] >> simp[] >>
     `∃n c. nc = n *, c` by metis_tac[npair_cases] >>
     fs[UPDATE_TAPE_ACT_STATE_TM_thm,NUM_TO_CELL_TO_NUM,FULL_ENCODE_TM_STATE] >>
-    `NUM_CELL (CELL_NUM c) = c` by metis_tac[CELL_NUM_LEM1,NUM_TO_CELL_TO_NUM] >> simp[] >> fs[] >>
+    `NUM_CELL (CELL_NUM c) = c` by metis_tac[CELL_NUM_LEM11,NUM_TO_CELL_TO_NUM] >> simp[] >> fs[] >>
     rfs[NUM_CELL_INJ] >>
     Cases_on `(STATE_TO_NUM tm.state = n) ∧ (NUM_CELL tm.tape_h = c)`  >> rw[]
-  >- (rw[] >> simp[]  >> simp[TM_ACT_LEM_1]  >> rfs[TM_ACT_LEM_1] >>
-     simp[updn_UPDATE_TAPE]  )
-  >- (rw[] >> simp[]  >> simp[TM_ACT_LEM_1]  >> rfs[TM_ACT_LEM_1] >>
-    `∃ a s. p ' (NUM_TO_STATE n,CELL_NUM c) = (s,a)` by metis_tac[pairTheory.pair_CASES] >>
-    first_x_assum(qspecl_then[`n`,`c`,`s`,`a`] mp_tac) >> simp[] >> rw[CELL_NUM_NUM_CELL_RW] >>
-    simp[ UPDATE_W_PROG_NIN_TM] )  )
- )
+    >- (fs[STATE_TO_NUM_def,REWRITE_RULE[STATE_TO_NUM_def] updn_UPDATE_TAPE] )
+    >- (`∃ a s. p ' (NUM_TO_STATE n,CELL_NUM c) = (s,a)` by metis_tac[pairTheory.pair_CASES] >>
+        first_x_assum(qspecl_then[`n`,`c`,`s`,`a`] mp_tac) >> simp[] >> rw[CELL_NUM_NUM_CELL_RW] >>
+        simp[UPDATE_TAPE_def,STATE_TO_NUM_def,NUM_TO_STATE_def] >>
+        Cases_on `(tm.state,tm.tape_h) ∈ FDOM p` >> simp[]
+        >- (Cases_on `tm.state.n = 0` >>simp[]
+            >- simp_tac bool_ss [FULL_ENCODE_IGNORES_PROGS, GSYM TM_fupdcanon]
+            >- (COND_CASES_TAC
+                >- (simp[DOMSUB_FAPPLY_THM ] >>
+                    `¬((<|n := n|> = tm.state) ∧ (CELL_NUM c = tm.tape_h))` by
+                    fs[STATE_TO_NUM_def,CELL_NUM_def,NUM_CELL_def] >>
+                    Cases_on `SND (p ' (tm.state,tm.tape_h))` >> rw[]
+    >- (`tm with <|state := FST (p ' (tm.state,tm.tape_h)); prog := p; tape_h := Z|> = tm with
+    <|prog := p; state := FST (p ' (tm.state,tm.tape_h));  tape_h := Z|>` by simp[] >>
+    asm_simp_tac bool_ss [] >>
+    `tm with <|state := FST (p ' (tm.state,tm.tape_h)); prog := p \\ (<|n := n|>,CELL_NUM c);
+    tape_h := Z|> = tm with
+    <|prog := p \\ (<|n := n|>,CELL_NUM c) ; state := FST (p ' (tm.state,tm.tape_h));
+    tape_h := Z|>` by simp[] >>asm_simp_tac bool_ss [] >>
+    rw[])
+   >-(`tm with <|state := FST (p ' (tm.state,tm.tape_h)); prog := p; tape_h := O|> = tm with
+   <|prog := p; state := FST (p ' (tm.state,tm.tape_h));  tape_h := O|>` by simp[] >>
+   asm_simp_tac bool_ss [] >>
+   `tm with <|state := FST (p ' (tm.state,tm.tape_h)); prog := p \\ (<|n := n|>,CELL_NUM c);
+   tape_h := O|> = tm with
+   <|prog := p \\ (<|n := n|>,CELL_NUM c) ; state := FST (p ' (tm.state,tm.tape_h));
+   tape_h := O|>` by simp[] >>asm_simp_tac bool_ss [] >>
+   rw[])
+   >- (`<|state := FST (p ' (tm.state,tm.tape_h)); prog := p; tape_l := []; tape_h := Z;
+     tape_r := tm.tape_h::tm.tape_r|> = 
+     <|prog := p; state := FST (p ' (tm.state,tm.tape_h));  tape_l := []; tape_h := Z;
+    tape_r := tm.tape_h::tm.tape_r|>` by simp[] >>
+    asm_simp_tac bool_ss [] >>
+    ` <|state := FST (p ' (tm.state,tm.tape_h)); prog := p \\ (<|n := n|>,CELL_NUM c);
+                                   tape_l := []; tape_h := Z;
+                                   tape_r := tm.tape_h::tm.tape_r|> =
+     <|prog := p \\ (<|n := n|>,CELL_NUM c) ; state := FST (p ' (tm.state,tm.tape_h));
+                                   tape_l := []; tape_h := Z;
+                                   tape_r := tm.tape_h::tm.tape_r|>` by simp[] >>
+    asm_simp_tac bool_ss [] >> rw[])
+    >- (`<|state := FST (p ' (tm.state,tm.tape_h)); prog := p; tape_l := TL tm.tape_l;
+                                   tape_h := HD tm.tape_l; tape_r := tm.tape_h::tm.tape_r|> =
+    <|prog := p; state := FST (p ' (tm.state,tm.tape_h));  tape_l := TL tm.tape_l;
+                                   tape_h := HD tm.tape_l; tape_r := tm.tape_h::tm.tape_r|>` by
+      simp[] >>
+                                                                     asm_simp_tac bool_ss [] >>
+    `<|state := FST (p ' (tm.state,tm.tape_h)); prog := p \\ (<|n := n|>,CELL_NUM c);
+                                   tape_l := TL tm.tape_l;
+                                   tape_h := HD tm.tape_l; tape_r := tm.tape_h::tm.tape_r|> =
+    <|prog := p \\ (<|n := n|>,CELL_NUM c) ; state := FST (p ' (tm.state,tm.tape_h));
+                                   tape_l := TL tm.tape_l;
+                                   tape_h := HD tm.tape_l;
+                                   tape_r := tm.tape_h::tm.tape_r|>` by simp[] >>
+    asm_simp_tac bool_ss [] >> rw[])
+    >- (`<|state := FST (p ' (tm.state,tm.tape_h)); prog := p; tape_l := tm.tape_h::tm.tape_l;
+                                   tape_h := Z; tape_r := []|> =
+    <|prog := p; state := FST (p ' (tm.state,tm.tape_h)); tape_l := tm.tape_h::tm.tape_l;
+                                   tape_h := Z; tape_r := []|>` by simp[] >>
+                                                                     asm_simp_tac bool_ss [] >>
+   `<|state := FST (p ' (tm.state,tm.tape_h)); prog := p \\ (<|n := n|>,CELL_NUM c);
+                                   tape_l := tm.tape_h::tm.tape_l; tape_h := Z; tape_r := []|> =
+     <|prog := p \\ (<|n := n|>,CELL_NUM c) ; state := FST (p ' (tm.state,tm.tape_h));
+                                   tape_l := tm.tape_h::tm.tape_l;
+                                   tape_h := Z; tape_r := []|>` by simp[] >>
+    asm_simp_tac bool_ss [] >> rw[])
+    >- (`<|state := FST (p ' (tm.state,tm.tape_h)); prog := p; tape_l := tm.tape_h::tm.tape_l;
+                                   tape_h := HD tm.tape_r;
+                                   tape_r := TL tm.tape_r|> =
+     <|prog := p; state := FST (p ' (tm.state,tm.tape_h)); tape_l := tm.tape_h::tm.tape_l;
+                                   tape_h := HD tm.tape_r;
+                                   tape_r := TL tm.tape_r|>` by simp[] >> asm_simp_tac bool_ss [] >>
+    `<|state := FST (p ' (tm.state,tm.tape_h)); prog := p \\ (<|n := n|>,CELL_NUM c);
+                                   tape_l := tm.tape_h::tm.tape_l; tape_h := HD tm.tape_r;
+                                   tape_r := TL tm.tape_r|> =
+     <|prog := p \\ (<|n := n|>,CELL_NUM c) ; state := FST (p ' (tm.state,tm.tape_h));
+                                   tape_l := tm.tape_h::tm.tape_l; tape_h := HD tm.tape_r;
+                                   tape_r := TL tm.tape_r|>` by simp[] >>
+    asm_simp_tac bool_ss [] >> rw[])   )
+
+
+                >- (fs[STATE_TO_NUM_def,CELL_NUM_def,NUM_CELL_def] >>
+                                     Cases_on `SND (p ' (tm.state,tm.tape_h))` >> rw[])
+               ) ) >- (simp_tac bool_ss [FULL_ENCODE_IGNORES_PROGS, GSYM TM_fupdcanon])  ) )
+
+                                      )
+
+(* I am sorry *)
+
 
 val nsnd0 = EVAL ``nsnd 0``
 
@@ -645,18 +757,26 @@ strip_tac >> SRW_TAC [][primrec_rules] >> SRW_TAC [][pr_cond_def] >>
 
 val primrec_tmstepf = Q.store_thm ("primerec_tmstepf",
 `primrec (pr1 (tmstepf p) ) 1`,
- Induct_on `CARD (FDOM p)` >- (rpt strip_tac >>
+Induct_on `CARD (FDOM p)`
+>- (rpt strip_tac >>
   `FDOM p = {}` by metis_tac[FDOM_FINITE,CARD_EQ_0] >> fs[FDOM_EQ_EMPTY] >>
   rw[Once tmstepf_def] >> qmatch_abbrev_tac`primrec f 1` >>
-  `f = proj 0` suffices_by simp[primrec_rules] >> simp[Abbr`f`,FUN_EQ_THM] >> Cases >>
-  simp[proj_def] >> rw[Once tmstepf_def]  )
-    >- (rpt strip_tac >>  MATCH_MP_TAC primrec_pr1  >> rw[Once tmstepf_def] >>
-      ` (OLEAST n.  (NUM_TO_STATE (nfst n),CELL_NUM (nsnd n)) ∈ FDOM p) <> NONE`
+  `f = Cn (pr2 npair) [zerof; Cn (pr1 nsnd) [proj 0]]` suffices_by
+  simp[primrec_rules,primrec_npair,primrec_nsnd] >>
+  simp[Abbr`f`,FUN_EQ_THM] >> Cases >>
+  simp[proj_def,nsnd_def] >> rw[Once tmstepf_def] >> simp[nsnd_def]  )
+>- (rpt strip_tac >>  MATCH_MP_TAC primrec_pr1  >> rw[Once tmstepf_def] >>
+` (OLEAST n.  (NUM_TO_STATE (nfst n),CELL_NUM (nsnd n)) ∈ FDOM p)  <> NONE`
         by (DEEP_INTRO_TAC(whileTheory.OLEAST_INTRO) >> simp[] >>
             `FDOM p <> {}` by (strip_tac >> fs[]) >>
             `∃a b. (a,b) IN FDOM p`  by metis_tac[SET_CASES,pairTheory.pair_CASES,IN_INSERT]>>
             qexists_tac`STATE_TO_NUM a *, NUM_CELL b` >> simp[] ) >>
-      `∃k. (OLEAST n.  (NUM_TO_STATE (nfst n),CELL_NUM (nsnd n)) ∈ FDOM p) = SOME k`
+   Cases_on `(OLEAST n. (NUM_TO_STATE (nfst n),CELL_NUM (nsnd n)) ∈ FDOM p ∧ nfst n ≠ 0) = NONE` >>
+   fs[]
+   >- (qexists_tac `Cn (pr2 npair) [zerof; Cn (pr1 nsnd) [proj 0]]` >> conj_tac
+      >- simp[primrec_rules,primrec_npair,primrec_nsnd]
+      >- (strip_tac >> simp[proj_def,nsnd_def]) )
+   >- ( `∃k. (OLEAST n.  (NUM_TO_STATE (nfst n),CELL_NUM (nsnd n)) ∈ FDOM p ∧ nfst n ≠ 0) = SOME k`
       by metis_tac[optionTheory.option_CASES] >> simp[] >> fs[OLEAST_EQ_SOME] >>
       `∃ s a. (p ' (NUM_TO_STATE (nfst k),CELL_NUM (nsnd k))) = (s,a)`
       by metis_tac[pairTheory.pair_CASES] >> simp[] >>
@@ -664,7 +784,7 @@ val primrec_tmstepf = Q.store_thm ("primerec_tmstepf",
       qabbrev_tac`q = p \\ (NUM_TO_STATE (nfst k),CELL_NUM (nsnd k))` >>
       `primrec (pr1 (tmstepf q)) 1` by fs[] >>
       `NUM_CELL (CELL_NUM (nsnd k)) = nsnd k`
-      by metis_tac[npair_11,npair,CELL_NUM_LEM1,NUM_TO_CELL_TO_NUM] >> fs[] >>
+      by metis_tac[npair_11,npair,CELL_NUM_LEM11,NUM_TO_CELL_TO_NUM] >> fs[] >>
       qabbrev_tac`snum = STATE_TO_NUM s` >> qabbrev_tac`anum = ACT_TO_NUM a` >>
       qexists_tac`Cn (proj 0)  [
      pr_cond (Cn (pr2 $*)  [Cn pr_eq [Cn (pr1 nfst) [proj 0] ; Cn (pr1 nfst) [K k] ];
@@ -672,7 +792,7 @@ val primrec_tmstepf = Q.store_thm ("primerec_tmstepf",
                                       Cn (pr1 nsnd) [K k] ] ] )
                  (Cn updn [K snum; K anum ; proj 0] )
                  (Cn (pr1 (tmstepf q)) [proj 0]  )
-             ] ` >> fs[primrec_of_tmstepf,primrec_tmstepf_form]
+             ] ` >> fs[primrec_of_tmstepf,primrec_tmstepf_form])
     )   )
 
 val tm_return_def = tDefine"tm_return"`
@@ -693,10 +813,47 @@ val un_nlist_def = tDefine"un_nlist"`
 
 
 
-val INITIAL_TM_NUM_def = Define`INITIAL_TM_NUM  = λn. ⟦INITIAL_TM FEMPTY (un_nlist (proj 0 n))⟧`
+val INITIAL_TM_NUM_def = Define`INITIAL_TM_NUM = (λl. ⟦INITIAL_TM FEMPTY (un_nlist (proj 0 l))⟧)`
 
 val RUN_NUM_def = Define`
 RUN_NUM p targs = Pr (INITIAL_TM_NUM) (Cn (pr1 (tmstepf p)) [proj 1]) targs`
+
+val INITIAL_TAPE_PROG = Q.store_thm("INITIAL_TAPE_PROG",
+`(INITIAL_TAPE_TM tm l) with prog := p = INITIAL_TAPE_TM (tm with prog := p) l `,
+Cases_on `l` >> simp[INITIAL_TAPE_TM_def])
+
+val UPDATE_TAPE_PROG = Q.store_thm("UPDATE_TAPE_PROG",
+`(tm.prog = p) ==> ((UPDATE_TAPE tm) with prog := p = UPDATE_TAPE tm)`,
+strip_tac >>simp[UPDATE_TAPE_def] >> rw[] >> Cases_on `SND (tm.prog ' (tm.state,tm.tape_h))` >>simp[TM_component_equality] )
+
+val UPDATE_PROG_CONSERVE = Q.store_thm("UPDATE_PROG_CONSERVE[simp]",
+`(UPDATE_TAPE tm).prog = tm.prog`,
+simp[UPDATE_TAPE_def] >> rw[] >> Cases_on `SND (tm.prog ' (tm.state,tm.tape_h))` >>simp[TM_component_equality])
+
+val RUN_PROG_CONSERVE = Q.store_thm("RUN_PROG_CONSERVE[simp]",
+`(RUN n tm).prog = tm.prog`,
+Induct_on `n` >> simp[FUNPOW_SUC])
+
+val RUN_PROG = Q.store_thm("RUN_PROG",
+`(tm.prog = p) ==> ((RUN n tm) with prog := p = RUN n tm)`,
+ simp[TM_component_equality] )
+
+val INITIAL_TAPE_TM_PROG = Q.store_thm("INITIAL_TAPE_TM_PROG[simp]",
+`(INITIAL_TAPE_TM tm args).prog = tm.prog`,
+Cases_on `args` >> simp[INITIAL_TAPE_TM_def] )
+
+val INITIAL_TM_PROG = Q.store_thm("INITIAL_TM_PROG[simp]",
+`(INITIAL_TM p args).prog = p`,
+ simp[INITIAL_TM_def])
+
+val RUN_NUM_corr = Q.store_thm("RUN_NUM_corr",
+`RUN_NUM p [t;args] = ⟦FUNPOW UPDATE_TAPE t (INITIAL_TM p (un_nlist args))⟧`,
+simp[RUN_NUM_def] >> Induct_on `t` >> fs[]
+    >- (simp[INITIAL_TM_NUM_def,INITIAL_TM_def] >>
+        ONCE_REWRITE_TAC[FULL_ENCODE_IGNORES_PROGS|> Q.INST [`p`|-> `ARB` ] |> SYM  ] >>
+        simp_tac bool_ss[INITIAL_TAPE_PROG] >>simp[] )
+    >- (simp[FUNPOW_SUC] >> rw[SIMP_RULE bool_ss[] tmstepf_update_equiv] >>
+        fs[RUN_PROG] ) )
 
 val tm_return_num_def = Define`
 tm_return_num = Pr (Cn (pr1 nsnd) [Cn (pr1 nsnd) [proj 0]])
@@ -891,8 +1048,6 @@ SRW_TAC [][pr_tl_en_con_def,primrec_rules] >>
         fs[primrec_nleng] >>  irule alt_Pr_rule >> rw[primrec_pr_tl_en_con_fun4] );
 
 
-(* Works up to here  *)
-(* WORK IN PROGRESS SECTION   *)
 val invtri_zero = Q.store_thm("invtri_zero[simp]",
 `invtri 0 = 0`,
 EVAL_TAC)
@@ -1118,30 +1273,138 @@ val tape_encode_corr_sym = Q.store_thm("tape_encode_corr_sym",
 `ENCODE_TM_TAPE tm = tape_encode [ENCODE tm.tape_l;NUM_CELL tm.tape_h;ENCODE tm.tape_r]`,
 fs[tape_encode_corr])
 
+
+(* Define correctly so it matches what it should *)
 val pr_INITIAL_TAPE_TM_NUM_def = Define`
 pr_INITIAL_TAPE_TM_NUM = pr_cond (Cn pr_eq [proj 1;zerof]) (proj 0) (Cn (pr2 npair)
-[Cn (pr1 nfst) [proj 0];Cn (pr2 npair) [Cn (pr1 nhd) [proj 1];Cn (pr1 ntl) [proj 1]] ])`
+[Cn (pr1 nfst) [proj 0];Cn (pr2 npair) [Cn (pr1 nhd) [proj 1];Cn (pr1 ntl) [proj 1]] ])`;
 
 val primrec_pr_INITIAL_TAPE_TM_NUM = Q.store_thm("primrec_pr_INITIAL_TAPE_TM_NUM[simp]",
 `primrec pr_INITIAL_TAPE_TM_NUM 2`,
-fs[pr_INITIAL_TAPE_TM_NUM_def] >> `0<2` by fs[] >>irule primrec_pr_cond >> rpt (irule primrec_cn >> rw[primrec_rules,primrec_pr_eq,primrec_nsnd,primrec_nfst] ) >>fs[primrec_proj] )
+fs[pr_INITIAL_TAPE_TM_NUM_def] >> `0<2` by fs[] >>irule primrec_pr_cond >> rpt (irule primrec_cn >> rw[primrec_rules,primrec_pr_eq,primrec_nsnd,primrec_nfst] ) >>fs[primrec_proj] );
 
 val pr_INITIAL_TM_NUM_def = Define`
 pr_INITIAL_TM_NUM = Cn (pr2 npair) [zerof;Cn tape_encode
  [Cn (pr1 nfst) [Cn pr_INITIAL_TAPE_TM_NUM [zerof;Cn concatWith_Z [proj 0]]];
   Cn (pr1 nfst) [Cn (pr1 nsnd) [Cn pr_INITIAL_TAPE_TM_NUM [zerof;Cn concatWith_Z [proj 0]]]];
-  Cn (pr1 nsnd) [Cn (pr1 nsnd) [Cn pr_INITIAL_TAPE_TM_NUM [zerof;Cn concatWith_Z [proj 0]]]]]]`
+  Cn (pr1 nsnd) [Cn (pr1 nsnd) [Cn pr_INITIAL_TAPE_TM_NUM [zerof;Cn concatWith_Z [proj 0]]]]]]`;
 
-val primrec_pr_INITIAL_TM_NUM = Q.store_thm("primrec_pr_INITIAL_TM_NUM[simp]",
-`primrec pr_INITIAL_TM_NUM 1`,
-SRW_TAC [][pr_INITIAL_TM_NUM_def,primrec_rules] >>
-rpt ( MATCH_MP_TAC primrec_cn >> SRW_TAC [][primrec_rules,concatWith_Z_thm,primrec_pr_INITIAL_TAPE_TM_NUM,primrec_tape_encode,primrec_npair,primrec_ntl,primrec_nhd]))
+val pr_ODD_def = Define`pr_ODD = pr_cond (Cn pr_eq [Cn pr_mod [proj 0;twof];onef]) onef zerof`
 
+val pr_ODD_corr = Q.store_thm("pr_ODD_corr",
+`pr_ODD [x] = if ODD x then 1 else 0`,
+fs[pr_ODD_def] >> Cases_on `ODD x` >- metis_tac[ODD_MOD_TWO_lem] >>
+`EVEN x` by metis_tac[EVEN_OR_ODD] >> fs[EVEN_MOD2]);
+
+val GENLIST_ZERO = Q.store_thm("GENLIST_ZERO",
+`(GENLIST a b = []) <=> (b=0)`,
+eq_tac >> fs[GENLIST] >> strip_tac >> Cases_on `b` >> fs[GENLIST] );
+
+val concatWith_Z_empty = Q.store_thm("concatWith_Z_empty",
+`(concatWith [Z] (MAP (GENLIST (K O)) args) = []) <=> ((args = []) ∨ (args = [0]))`,
+eq_tac >- (strip_tac >> Cases_on `MAP (GENLIST (K O)) args` >> rfs[concatWith_def] >>
+      Cases_on `t` >> rfs[concatWith_def] >> `GENLIST (K O) x0 = []` by fs[] >> fs[GENLIST_ZERO])
+       >- (strip_tac >> rw[concatWith_def]));
+
+val head_concatWith = Q.store_thm("head_concatWith",
+`((l<> []) ∧ (HD l <> [])) ==> (HD (concatWith a l) = HD (HD l))`,
+strip_tac >> Cases_on `l` >> fs[concatWith_def] >> Cases_on `t` >> fs[concatWith_def,HD] >>
+                                 Cases_on `h` >> fs[])
+
+val head_nil_concatWith = Q.store_thm("head_nil_concatWith[simp]",
+`HD (concatWith [a] ([]::b::c)) = a`,
+rw[concatWith_def])
+
+val odd_encode_hd_concat = Q.store_thm("odd_encode_hd_concat",
+`(concatWith [Z] (MAP (GENLIST (K O)) args) <> []) ==> (NUM_CELL (HD (concatWith [Z] (MAP (GENLIST (K O)) args))) = 1 - pr_eq [proj 0 args;0])`,
+strip_tac >> fs[concatWith_Z_empty]
+          >> Cases_on `args` >- rw[concatWith_def] >> Cases_on `h = 0` >> simp[proj_def]>>
+          Cases_on `MAP (GENLIST (K O)) t`>> simp[]
+          >- (`t = []` by fs[MAP_EQ_NIL] >> rw[]) >> simp[concatWith_def]
+          >- (`∃h'. h = SUC h'` by metis_tac[num_CASES] >> rw[] >> fs[HD_GENLIST])
+          >- (`∃h'. h = SUC h'` by metis_tac[num_CASES] >> rw[] >> fs[GENLIST_CONS])  )
 
 val nfst_zero = Q.store_thm("nfst_zero[simp]", `nfst 0 = 0`, EVAL_TAC)
 val nsnd_zero = Q.store_thm("nsnd_zero[simp]", `nsnd 0 = 0`, EVAL_TAC)
 val nhd_zero = Q.store_thm("nfst_zero[simp]", `nhd 0 = 0`, EVAL_TAC)
 val ntl_zero = Q.store_thm("nsnd_zero[simp]", `ntl 0 = 0`, EVAL_TAC)
+
+val num_cell_encode_hd_concat = Q.store_thm("num_cell_encode_hd_concat",
+`(concatWith [Z] (MAP (GENLIST (K O)) args) <> []) ==> (NUM_CELL (HD (concatWith [Z] (MAP (GENLIST (K O)) args))) = 1 - pr_eq [ nhd  (nlist_of args);0])`,
+rw[odd_encode_hd_concat] >> Cases_on `args` >> simp[nhd_thm]  )
+
+val encode_concat_def = tDefine "encode_concat" `
+    (encode_concat 0 = 0) ∧
+    (encode_concat args = ((2** (nhd args)) - 1) +
+                          (2* ((2** (nhd args))) * (encode_concat (ntl args))))`
+(qexists_tac `$<` >> conj_tac >- simp[prim_recTheory.WF_LESS] >> strip_tac >>
+`ntl (SUC v) <= v` by simp[ntl_suc_less] >> `v < SUC v` by simp[prim_recTheory.LESS_SUC_REFL]>>
+rw[])
+
+val encode_tl_concat_def = Define`encode_tl_concat args = DIV2 (encode_concat args)`
+
+val ENCODE_GENLIST_p_Z = Q.store_thm("ENCODE_GENLIST_p_Z",
+`ENCODE (GENLIST (K O) h ++ [Z] ++ b) = ((2**h) - 1) + (2*((2**h))*(ENCODE b))`,
+Induct_on `h` >> simp[ENCODE_def] >> simp[GENLIST_CONS] >> simp[ENCODE_def] >>rw[EXP] >>
+`2 * (2 ** h − 1 + 2 * (ENCODE b * 2 ** h)) = 2*2 ** h − 2*1 + 4 * (ENCODE b * 2 ** h)` by fs[]>>
+rw[] >> `2<=2*2**h` by (rpt (pop_assum kall_tac) >> Induct_on `h` >> simp[])  >> simp[])
+
+val ENCODE_GENLIST_O = Q.store_thm("ENCODE_GENLIST_O",
+`ENCODE (GENLIST (K O) h) = 2 ** h − 1`,
+Induct_on `h` >> simp[ENCODE_def,GENLIST_CONS,EXP] >> `1<=2**h` suffices_by simp[] >>
+          `0<2**h` suffices_by decide_tac >> simp[])
+
+val encode_concat_corr = Q.store_thm("encode_concat_corr",
+`ENCODE (concatWith [Z] (MAP (GENLIST (K O)) args)) = encode_concat (nlist_of args)`,
+Induct_on `args` >> fs[concatWith_def,ENCODE_def,encode_concat_def] >> strip_tac >>
+`nhd (ncons h (nlist_of args)) = h` by simp[nhd_thm] >> `ntl (ncons h (nlist_of args)) =
+nlist_of args` by simp[ntl_thm] >> `ncons h (nlist_of args) <> 0` by simp[ncons_not_nnil] >>
+`∃ n0. ncons h (nlist_of args) = SUC n0 ` by metis_tac[num_CASES] >>rw[encode_concat_def] >>
+full_simp_tac bool_ss[] >>
+Cases_on `args` >> simp[concatWith_def] >- simp[encode_concat_def,ENCODE_GENLIST_O] >>
+simp[ENCODE_GENLIST_p_Z] >> fs[])
+
+val pr_INITIAL_TM_NUM_def = Define`
+pr_INITIAL_TM_NUM = Cn (pr2 npair) [zerof;Cn tape_encode
+                                             [zerof;
+                                    Cn (pr2 $-) [onef ;Cn pr_eq [Cn (pr1 nhd) [proj 0];zerof]];
+                                              Cn (pr1 encode_tl_concat) [proj 0]]]`
+
+val encode_concat_list_rec = Q.store_thm("encode_concat_list_rec",
+`encode_concat n = nel n  (list_rec_comb (Cn (pr2 $+) [Cn (pr1 PRE) [Cn (pr2 $EXP) [twof;proj 0]];
+                             Cn (pr2 $*) [twof;Cn (pr2 $*) [proj 2;Cn (pr2 $EXP) [twof;proj 0]]]])0  n)`,
+rw[list_rec_comb_corr] >> `∃l.  n =  nlist_of l` by metis_tac[nlist_of_onto] >> rw[] >> Induct_on `l` >> simp[LIST_REC_def,encode_concat_def,un_nlist_def] >> strip_tac >> `ncons h (nlist_of l) <> 0` by simp[ncons_not_nnil] >>
+`∃ n0. ncons h (nlist_of l) = SUC n0 ` by metis_tac[num_CASES] >>rw[encode_concat_def] >>
+full_simp_tac bool_ss[] >> pop_assum (SUBST_ALL_TAC o SYM) >>simp[nel_nlist_of,LIST_REC_def] )
+
+val pr_encode_concat_def = Define`pr_encode_concat = Cn (pr2 nel) [proj 0;
+  Cn (pr1 (list_rec_comb (Cn (pr2 $+) [Cn (pr1 PRE) [Cn (pr2 $EXP) [twof;proj 0]];
+  Cn (pr2 $*) [twof;Cn (pr2 $*) [proj 2;Cn (pr2 $EXP) [twof;proj 0]]]]) 0)) [proj 0]]`
+
+val pr_encode_tl_concat_def = Define`pr_encode_tl_concat = Cn (pr1 DIV2) [Cn (pr2 nel) [proj 0;
+   Cn (pr1 (list_rec_comb (Cn (pr2 $+) [Cn (pr1 PRE) [Cn (pr2 $EXP) [twof;proj 0]];
+   Cn (pr2 $*) [twof;Cn (pr2 $*) [proj 2;Cn (pr2 $EXP) [twof;proj 0]]]]) 0)) [proj 0]]]`
+
+
+val primrec_exp = Q.store_thm("primrec_exp",
+`primrec (pr2 $**) 2`,
+ irule primrec_pr2 >>qexists_tac `pr_exp` >> conj_tac >-simp[primrec_pr_exp] >> simp[pr_exp_def]>>
+Induct >> Induct >> simp[] >> rw[EXP])
+
+val primrec_pr_INITIAL_TM_NUM = Q.store_thm("primrec_pr_INITIAL_TM_NUM[simp]",
+`primrec pr_INITIAL_TM_NUM 1`,
+SRW_TAC [][pr_INITIAL_TM_NUM_def,primrec_rules] >>
+        rpt ( MATCH_MP_TAC primrec_cn >> SRW_TAC [][primrec_rules,concatWith_Z_thm,primrec_pr_INITIAL_TAPE_TM_NUM,primrec_tape_encode,primrec_npair,primrec_ntl,primrec_nhd]) >>
+        irule primrec_pr1 >> qexists_tac `pr_encode_tl_concat` >> conj_tac
+        >- (rw[pr_encode_tl_concat_def] >>rpt (irule primrec_cn >> rw[primrec_rules,primrec_nel] )>-
+(`primrec (Cn (pr2 $+)
+             [Cn (pr1 PRE) [Cn (pr2 $** ) [twof; proj 0]];
+              twof *. (proj 2 *. Cn (pr2 $** ) [twof; proj 0])]) 3` suffices_by
+        rw[primrec_list_rec_comb] >> rpt (irule primrec_cn >> rw[primrec_rules,primrec_nel] ) >>
+        simp[primrec_exp,primrec_div2]) >> simp[primrec_div2] )
+        >- (strip_tac >> simp[encode_concat_list_rec] >> `∃l.  n =  nlist_of l` by metis_tac[nlist_of_onto] >> rw[] >> Induct_on `l` >> simp[list_rec_comb_def,encode_tl_concat_def,encode_concat_def,nlist_of_def,pr_encode_concat_def] >- simp[pr_encode_concat_def,pr_encode_tl_concat_def,list_rec_comb_def] >> strip_tac >> simp[pr_encode_tl_concat_def,encode_concat_list_rec]   ) )
+
+
 
 val nhd_nlist_of = Q.store_thm("nhd_nlist_of[simp]",
 `nhd (nlist_of (h::t)) = h`,
@@ -1164,40 +1427,127 @@ strip_tac >> eq_tac >> rw[tape_encode_thm]
          >- (CCONTR_TAC >> rfs[] >> `ODD (SUC (2* c))` by fs[ODD_DOUBLE] >> `EVEN (2*f)` by
            fs[EVEN_DOUBLE] >> rfs[EVEN_AND_ODD] >> metis_tac[EVEN_AND_ODD])  )
 
-(* currently working on 
+
+val ENCODE_TL_concatWith = Q.store_thm("ENCODE_TL_concatWith",
+`(concatWith [Z] (MAP (GENLIST (K O)) args) = h::t) ==> (ENCODE t = encode_tl_concat (nlist_of args))`,
+rw[] >> simp[encode_tl_concat_def] >> `ENCODE t = ENCODE (TL (concatWith [Z] (MAP (GENLIST (K O)) args)))`
+by simp[] >> metis_tac[encode_concat_corr,ENCODE_TL_DIV2])
+
 val primrec_INITIAL_TM_NUM = Q.store_thm("primrec_INITIAL_TM_NUM",
 `primrec INITIAL_TM_NUM 1`,
 `INITIAL_TM_NUM = pr_INITIAL_TM_NUM` suffices_by fs[primrec_pr_INITIAL_TM_NUM] >>
  fs[FUN_EQ_THM] >> strip_tac >>
- fs[INITIAL_TM_NUM_def,INITIAL_TM_def,un_nlist_def,INITIAL_TAPE_TM_def,FULL_ENCODE_TM_def,STATE_TO_NUM_def] >> Cases_on `(concatWith [Z] (MAP (GENLIST (K O)) (un_nlist (proj 0 x))))` >>
+ fs[INITIAL_TM_NUM_def,INITIAL_TM_def,un_nlist_def,INITIAL_TAPE_TM_def,FULL_ENCODE_TM_def,STATE_TO_NUM_def,pr_INITIAL_TM_NUM_def,tape_encode_corr_sym]
+>> Cases_on `(concatWith [Z] (MAP (GENLIST (K O)) (un_nlist (proj 0 x))))` >>
 fs[INITIAL_TAPE_TM_def]  >>
-fs[pr_INITIAL_TM_NUM_def,pr_INITIAL_TAPE_TM_NUM_def,tape_encode_corr,concatWith_Z_corr]>>
-Cases_on `nlist_of (concatWith [0] (MAP un_nlist (un_nlist (proj 0 x))))` >> rw[] >-
-(`tape_encode [0;0;0] = tape_encode [ENCODE [];NUM_CELL Z;ENCODE []]` by
- fs[ENCODE_def,NUM_CELL_def] >> asm_simp_tac list_ss [tape_encode_corr_sym,EQ_SYM] >> fs[] )
->- (fs[tape_encode_corr_sym,ENCODE_def] >> fs[tape_encode_eq] >> )
->- (contra)
->- (fs[tape_encode_corr_sym] >> rw[nhd_nlist_of,ENCODE_def] )
-    )
+fs[pr_INITIAL_TM_NUM_def,pr_INITIAL_TAPE_TM_NUM_def,tape_encode_corr,concatWith_Z_corr]
+>- (`∃l. proj 0 x = nlist_of l` by metis_tac[nlist_of_onto] >>fs[]>>
+    `(l = []) ∨ (l = [0])` by rfs[concatWith_Z_empty] >> fs[encode_tl_concat_def,encode_concat_def,ENCODE_def,DIV2_def,ncons_def]  >>EVAL_TAC )
+>- (simp[ENCODE_def] >> `ENCODE t = encode_tl_concat (proj 0 x)` by
+(metis_tac[ENCODE_TL_concatWith,nlist_of_unnlist,un_nlist_nlist_of_inv]) >>
+simp[ENCODE_TL_concatWith] >>
+`NUM_CELL h = NUM_CELL (HD (concatWith [Z] (MAP (GENLIST (K O)) (un_nlist (proj 0 x)))))` by
+simp[] >> simp[odd_encode_hd_concat] >>
+`nB (proj 0 (un_nlist (proj 0 x)) ≠ 0) = nB (nhd (proj 0 x) ≠ 0)` suffices_by simp[]  >> rw[] >>
+Cases_on `x` >> simp[un_nlist_def] >> `∃l.  h' =  nlist_of l` by metis_tac[nlist_of_onto] >> rw[]>> Cases_on `l` >> simp[]) )
+
+
+
+val RUN_NUM_p = Q.store_thm("RUN_NUM_p",
+`RUN_NUM p = Pr INITIAL_TM_NUM (Cn (pr1 (tmstepf p)) [proj 1]) `,
+simp[FUN_EQ_THM,RUN_NUM_def]);
 
 val primrec_RUN_NUM = Q.store_thm("primrec_RUN_NUM",
 `primrec (RUN_NUM p) 2`,
-rw[RUN_NUM] >> fs[primrec_INITIAL_TM_NUM,primrec_cn,primrec_tmstepf,alt_Pr_rule])
+fs[RUN_NUM_p] >> irule alt_Pr_rule >- fs[primrec_INITIAL_TM_NUM] >> irule primrec_cn
+  >- (fs[primrec_rules])
+  >> fs[primrec_tmstepf]);
+
+val Pr_thm_one = Q.store_thm("Pr_thm_one",
+`(Pr b r (1::t) = r (0::Pr b r (0::t)::t))`,
+rw[Pr_thm] >> `Pr b r (1::t) = Pr b r ((SUC 0)::t)` by metis_tac[ONE] >> rw[])
+
+val zero_less_nB = Q.store_thm("zero_less_nB[simp]",
+`(0 < nB A) <=> A`,
+Cases_on `A` >> fs[])
+
+
+val recfn_rulesl = CONJUNCTS recfn_rules
+val recfnCn = save_thm("recfnCn", List.nth(recfn_rulesl, 3))
+val recfnPr = save_thm("recfnPr", List.nth(recfn_rulesl, 4))
+val recfnMin = save_thm("recfnMin", List.nth(recfn_rulesl, 5))
+
+val STATE_TO_NUM_EQ = Q.store_thm("STATE_TO_NUM_EQ[simp]",
+`(STATE_TO_NUM a = STATE_TO_NUM b) <=> (a=b)`,
+fs[STATE_TO_NUM_def] >> simp[state_component_equality]);
+
+
+
+(* Probably need to include a 'tape reset' type function, ie tm_return_num *)
+val recfn_tm_def = Define`
+recfn_tm p =  (recCn (SOME o (RUN_NUM p)) [minimise (SOME o
+              (Cn pr_eq [Cn (RUN_NUM p) [proj 0;proj 1];Cn (RUN_NUM p) [Cn succ [proj 0];
+                                         proj 1   ] ] )  ) ;SOME o (proj 0)]) `
+
+val recfn_tm_recfn = Q.store_thm("recfn_tm_recfn",
+`recfn (recfn_tm p) 1`,
+rw[recfn_tm_def] >> fs[primrec_RUN_NUM,primrec_recfn] >> irule recfnCn >> rw[recfn_rules]
+  >- (irule recfnMin >> fs[] >> irule primrec_recfn >> rpt (irule primrec_cn >> rw[primrec_rules,primrec_pr_eq,primrec_RUN_NUM,primrec_pr_add] ))
+  >- (fs[primrec_RUN_NUM,primrec_recfn]))
+
+(* works up to here *)
+
+(*
 
 val recfn_tm_def = Define`
 recfn_tm p n = (recCn (SOME o tm_return_num)
   [recCn tm_log_num [SOME o (RUN_NUM p) ];SOME o (RUN_NUM p)])
   [minimise (SOME o
-    (pr_cond (Cn pr_eq [Cn (RUN_NUM p) [proj 0];Cn (RUN_NUM p) [Cn (pr2 $+) [proj 0;onef]
-                    ] ] ) ) ) n; proj 0 n]`
+    (pr_cond (Cn pr_eq [Cn (RUN_NUM p) [proj 0];Cn (RUN_NUM p) [Cn succ [proj 0]
+                    ] ] ) ) ) n; proj 0 n]`;
 
-val recfn_tm_recfn = Q.store_thm("recfn_tm_recfn",
-`recfn (recfn_tm p) 1`,
-fs[primrec_tmstepf,primrec_recfn,INITIAL_TM_NUM_PR,primrec_rules] )
+val tm_return_num_corr = Q.store_thm("tm_return_num_corr",
+`tm_return tm = tm_return_num [(LENGTH tm.tape_r) + 1;⟦tm⟧]`,
+Induct_on `LENGTH tm.tape_r` >> fs[tm_return_num_def]
+          >- (rpt strip_tac >>  fs[Pr_thm_one] >> )
+          >>fs[tm_return_def])
+*)
+
+(* 
+val UPDATE_TAPE_HALTED = Q.store_thm("UPDATE_TAPE_HALTED[simp]",
+`(HALTED tm) ==> (UPDATE_TAPE tm = tm)`,
+rw[] >> fs[UPDATE_TAPE_def,HALTED_def] >> `tm.state =  <|n := 0|>` by fs[] )
+
+val run_num_halted = Q.store_thm("run_num_halted",
+`∃n. HALTED (RUN n (INITIAL_TM p args)) ==>
+ (RUN_NUM p [m; nlist_of args] = RUN_NUM p [SUC m; nlist_of args]) `,
+rw[RUN_NUM_corr] >> qexists_tac `m` >> rw[] >> rfs[FUNPOW_SUC] )
+
+
+(* This cannot be true for the same reason as above *)
+val minimise_corr = Q.store_thm("minimise_corr",
+`minimise (SOME ∘ Cn pr_eq [Cn (RUN_NUM p) [proj 0; proj 1];
+                            Cn (RUN_NUM p) [Cn succ [proj 0]; proj 1]]) [nlist_of args]
+                    =(OLEAST n. HALTED (RUN n (INITIAL_TM p args)))`,
+simp[whileTheory.OLEAST_def,minimise_def] >> rw[]
+    >- (fs[HALTED_def] >> rw[RUN_NUM_corr] >> simp[] >>SELECT_ELIM_TAC >>
+        rw[] >- (qexists_tac `n'` >> rfs[RUN_NUM_corr])
+        >- (numLib.LEAST_ELIM_TAC >> rw[] >- (qexists_tac `n` >> rfs[])
+           >- () ) )
+    >- (rfs[RUN_NUM_corr])
+    >- () )
+
+
+
 
 val main_eq_thm = Q.store_thm("main_eq_thm",
 `∀p. ∃f. (recfn f 1) ∧ (∀ args. tm_fn p args = f [nlist_of args])`,
-strip_tac >> qexists_tac`recfn_tm p` >- (fs[recfn_tm_recfn]) >> strip_tac >> )
+strip_tac >> qexists_tac`recfn_tm p` >> conj_tac >- fs[recfn_tm_recfn] >>
+          strip_tac >> fs[tm_fn_def,recfn_tm_def] >>
+          Cases_on `(OLEAST n. HALTED (RUN n (INITIAL_TM p args)))` >>
+          fs[optionTheory.OPTION_MAP_DEF] >> rw[RUN_NUM_corr] >> fs[recCn_def]
+          >- (fs[minimise_def] >> rpt strip_tac >> rfs[RUN_NUM_corr] >> qexists_tac `0` >>)
+          >- (rw[] >- () >- () ) )
 
 
 *)
